a

proof/garble/proofGarble.ec
@@ -58,9 +58,15 @@ clone Mean as MeanBool with
   op d = Dbool.dbool,
   op support = Set.add false (Set.add true Set.empty).
 
+op integers : int -> int -> int set.
+
+axiom integers_neg : forall (x y:int), x > y => integers x y = Set.empty.
+axiom integers_pos : forall (x y:int), x <= y => integers x y = add y (integers x (y-1)).
+
 clone Mean as MeanInt with
   type base = int,
-  op d = Dinter.dinter 0 (borne).
+  op d = Dinter.dinter 0 (borne),
+  op support = integers 0 borne.
 
 module DkcWorkAdv(Adv:DKC.Adv) = {
   module Game = DKC.Game(DKC.Dkc, Adv)
@@ -86,18 +92,17 @@ module DkcWork(Adv:DKC.Adv) : MeanBool.Worker = {
 lemma DkcExp : forall (M<:DKC.Exp),
   equiv[M.work~M.work:(glob M){1}=(glob M){2}==>res{1}=res{2}].
 proof.
-admit. (*
-intros M;fun true;trivial. *)
+intros _;fun true;progress assumption.
 save.
 
-(*
+
 lemma DkcWork :
   forall b,
   forall &m,
-    forall (Adv<:DKC.Adv {DKC.Dkc}),
+    forall (Adv<:DKC.Adv {DKC.Dkc, DKC.Game}),
       DKC.Dkc.b{m} = b =>
   Pr[DkcWorkAdv(Adv).work()@ &m:res] = 
-    Pr[DkcWork(Adv).work(b)@ &m:res] =
+    Pr[DkcWork(Adv).work(b)@ &m:res].
 proof.
   intros b &m Adv h.
   cut eq : equiv[DkcWorkAdv(Adv).work ~ DkcWork(Adv).work
@@ -107,13 +112,11 @@ proof.
   call ((glob DKC.Game(DKC.Dkc,Adv)){1} = (glob DKC.Game(DKC.Dkc,Adv)){2}) (res{1}=res{2}).
   apply (DkcExp (<:DKC.Game(DKC.Dkc,Adv))).
   call ((glob Adv){1} = (glob Adv){2}) (res{1}=res{2}/\(glob Adv){1} = (glob Adv){2}).
-  fun true;trivial.
+  fun true;progress assumption.
   wp.
-  skip. progress.
-  equiv_deno eq.
-  progress assumption.
-  trivial.
-save.*)
+  skip;progress.
+  equiv_deno eq;progress assumption.
+save.
 
 theory AdvEsp.
 
@@ -133,7 +136,7 @@ module AdvWork(Adv:Garble.Adv) : MeanInt.Worker = {
 
 lemma AdvEsp :
   forall &m,
-    forall (Adv<:Garble.Adv),
+    forall (Adv<:Garble.Adv{DKC.Dkc,AdvGarble.Adv,DKC.Game}),
       forall c, c = b =>
       Pr[DkcWork(AdvGarble.Adv(Adv)).work(c)@ &m:res] =
         (sum (lambda l, (1%r / (borne + 1)%r) * Pr[AdvWork(Adv).work(l)@ &m:res]) MeanInt.support).
@@ -171,16 +174,13 @@ apply (Fun.extensionality<:real, int> (lambda (x:int),
 else
   0%r)) (lambda (x:int), (mu_x MeanInt.d x * Pr[AdvWork(Adv).work(x) @ &m :res{hr}])) _).
 intros x.
-case (mem x MeanInt.support = true).
+case (mem x MeanInt.support = true);last trivial.
 intros hh.
 delta MeanInt.d.
-rewrite (Dinter.mu_x_def_in 0 borne x _).
-trivial.
-rewrite (_:borne - 0 + 1 = borne + 1).
-trivial.
+rewrite (Dinter.mu_x_def_in 0 borne x _);first trivial.
+rewrite (_:borne - 0 + 1 = borne + 1);first trivial.
 rewrite hh.
 progress.
-trivial.
 rewrite lem.
 apply (MeanInt.Mean &m (<:AdvWork(Adv))).
 save.
@@ -192,7 +192,7 @@ clone AdvEsp as AdvEspFalse with op b = false.
 
 lemma DkcEsp :
   forall &m,
-    forall (Adv<:DKC.Adv {DKC.Dkc}),
+    forall (Adv<:DKC.Adv {DKC.Dkc, DKC.Game}),
       Pr[DKC.Game(DKC.Dkc, Adv).main()@ &m:res] = 
         (Pr[DkcWork(Adv).work(true)@ &m:res] +
            Pr[DkcWork(Adv).work(false)@ &m:res]) / 2%r.
@@ -208,23 +208,35 @@ proof.
       inline DKC.Dkc.preInit.
       inline DkcWork(Adv).work.
       wp.
-      cut prelem : (forall (M<:DKC.Exp), equiv[M.work~M.work:(glob M){1}=(glob M){2}==>res{1}=res{2}]);[intros M;fun true;trivial|].
-      call ((glob DKC.Game(DKC.Dkc, Adv)){1}=(glob DKC.Game(DKC.Dkc, Adv)){2}) (res{1}=res{2}).
-      apply (prelem (<:DKC.Game(DKC.Dkc, Adv))).
+      cut prelem : (forall (M<:DKC.Exp), equiv[M.work~M.work:(glob M){1}=(glob M){2}==>res{1}=res{2}]);
+        first (intros M;fun true;by progress).
+      call ((glob DKC.Game(DKC.Dkc, Adv)){1}=(glob DKC.Game(DKC.Dkc, Adv)){2}) (res{1}=res{2});
+        first apply (prelem (<:DKC.Game(DKC.Dkc, Adv))).
       wp.
-      call ((glob Adv){1} = (glob Adv){2}) ((glob Adv){1} = (glob Adv){2});[fun true;trivial|].
-      wp.
-      rnd.
-      skip. progress assumption.
+      call ((glob Adv){1} = (glob Adv){2}) ((glob Adv){1} = (glob Adv){2});first (fun true;by progress).
+      wp;rnd;skip;by (progress assumption).
     equiv_deno eq;progress assumption;trivial.
   rewrite pr.
   rewrite (MeanBool.Mean &m (<:DkcWork(Adv))).
-  admit.
+  delta MeanBool.support.
+  rewrite (sum_add<:bool> (lambda (x : MeanBool.base),
+     mu_x MeanBool.d x * Pr[DkcWork(Adv).work(x) @ &m : res{hr}]) (add true Set.empty) false _);first trivial.
+  rewrite (sum_add<:bool> (lambda (x : MeanBool.base),
+     mu_x MeanBool.d x * Pr[DkcWork(Adv).work(x) @ &m : res{hr}]) Set.empty true _);first trivial.
+  rewrite (sum_nil<:bool> (lambda (x : MeanBool.base),
+     mu_x MeanBool.d x * Pr[DkcWork(Adv).work(x) @ &m : res{hr}])).
+  simplify.
+  delta MeanBool.d.
+  rewrite (Dbool.mu_x_def false).
+  rewrite (Dbool.mu_x_def true).
+  generalize Pr[DkcWork(Adv).work(false) @ &m : res{hr}].
+  generalize Pr[DkcWork(Adv).work(true) @ &m : res{hr}].
+  trivial.
 save.
 
 lemma RelDkcGarble :
   forall &m,
-    forall (Adv<:Garble.Adv{DKC.Dkc}),
+    forall (Adv<:Garble.Adv{DKC.Dkc,DKC.Game,AdvGarble.Adv}),
       Pr[Garble.Game(Garble.PrvInd(RandGarble), Adv).main()@ &m:res] =
         2%r * borne%r * Pr[DKC.Game(DKC.Dkc, AdvGarble.Adv(Adv)).main()@ &m:res]
           + 1%r / 2%r - borne%r.
@@ -233,6 +245,91 @@ proof.
   rewrite (DkcEsp &m (<:AdvGarble.Adv(Adv))).
   rewrite (AdvEspTrue.AdvEsp &m (<:Adv) true).
   rewrite (AdvEspFalse.AdvEsp &m (<:Adv) false).
+
+(**Remove Pr*)
+  cut introF : (exists (f:int->real), (forall (l:int), (f l) =
+    Pr[AdvEspTrue.AdvWork(Adv).work(l) @ &m : res{hr}]));first
+    (exists (lambda (l:int), Pr[AdvEspTrue.AdvWork(Adv).work(l) @ &m : res{hr}]);
+     simplify;split).
+  elim introF.
+  intros f fv.
+  rewrite (_:(lambda (l : int),
+       1%r / (Int.(+) borne 1)%r *
+       Pr[AdvEspTrue.AdvWork(Adv).work(l) @ &m : res{hr}]) = lambda (l : int),
+       1%r / (Int.(+) borne 1)%r * (f l));
+    first (apply extensionality;delta (==);simplify;intros l;rewrite (fv l);split).
+(**End Remove Pr*)
+
+(**Remove Pr*)
+  cut introG : (exists (g:int->real), (forall (l:int), (g l) =
+    Pr[AdvEspFalse.AdvWork(Adv).work(l) @ &m : res{hr}]));first
+    (exists (lambda (l:int), Pr[AdvEspFalse.AdvWork(Adv).work(l) @ &m : res{hr}]);
+     simplify;split).
+  elim introG.
+  intros g gv.
+  rewrite (_:(lambda (l : int),
+       1%r / (Int.(+) borne 1)%r *
+       Pr[AdvEspFalse.AdvWork(Adv).work(l) @ &m : res{hr}]) = lambda (l : int),
+       1%r / (Int.(+) borne 1)%r * (g l));
+    first (apply extensionality;delta (==);simplify;intros l;rewrite (gv l);split).
+(**End Remove Pr*)
+
+(**Remove Pr*)
+cut valf0 : (f 0 = Pr[Game(PrvInd(RandGarble), Adv).main() @ &m : res{hr}]).
+  admit.
+rewrite <- valf0.
+(**End Remove Pr*)
+
+trivial.
+
+  rewrite (sum_rm<:int>
+   (lambda (l : int), 1%r / (Int.(+) borne 1)%r * (f l))
+   MeanInt.support
+   0 _);first trivial.
+  rewrite (sum_rm<:int>
+   (lambda (l : int), 1%r / (Int.(+) borne 1)%r * (g l))
+   MeanInt.support
+   borne _);first trivial.
+trivial.
+rewrite ( _ :
+(lambda (l : int), 1%r / (Int.(+) borne 1)%r * (f l)) 0 +
+sum (lambda (l : int), 1%r / (Int.(+) borne 1)%r * (f l)) (rm 0 MeanInt.support) +
+((lambda (l : int), 1%r / (Int.(+) borne 1)%r * (g l)) borne +
+sum (lambda (l : int), 1%r / (Int.(+) borne 1)%r * (g l)) (rm borne MeanInt.support))
+=
+(lambda (l : int), 1%r / (Int.(+) borne 1)%r * (g l)) borne +
+(lambda (l : int), 1%r / (Int.(+) borne 1)%r * (f l)) 0 +
+(sum (lambda (l : int), 1%r / (Int.(+) borne 1)%r * (f l)) (rm 0 MeanInt.support) +
+sum (lambda (l : int), 1%r / (Int.(+) borne 1)%r * (g l)) (rm borne MeanInt.support))
+
+);trivial.
+
+  rewrite (sum_chind<:int>
+    (lambda (l : int),
+       1%r / (Int.(+) borne 1)%r *
+       Pr[AdvEspTrue.AdvWork(Adv).work(l) @ &m :res{hr}])
+    (lambda (x:int), x - 1)
+    (lambda (x:int), x + 1)
+    (rm 0 MeanInt.support) _);first trivial.
+  simplify.
+  rewrite (_ : 
+    (map (lambda (x : int), x-1) (rm 0 MeanInt.support)) =
+    (rm borne MeanInt.support)
+    ).
+  delta MeanInt.support.
+  apply (Induction.induction
+(lambda i, map (lambda (x : int), Int.(-) x 1) (rm 0 (integers 0 i)) =
+rm i (integers 0 i)) _ _ borne _);trivial.
+
+  rewrite (sum_add<:int>
+    (lambda (l : int),
+       1%r / (Int.(+) borne 1)%r *
+       Pr[AdvEspTrue.AdvWork(Adv).work((l + 1)) @ &m :res{hr}])
+    (lambda (l : int),
+       1%r / (Int.(+) borne 1)%r *
+       Pr[AdvEspFalse.AdvWork(Adv).work(l) @ &m :res{hr}])
+    (rm borne MeanInt.support)).
+  simplify.
   admit.
 (*
 cut test : (forall l, Pr[AdvEspFalse.AdvWork(Adv).work(l) @ &m : res{hr}] = 1%r - Pr[AdvEspFalse.AdvWork(Adv).work(l) @ &m : ! res{hr}]).
