proof/myset.ec
@@ -2,28 +2,153 @@ require import Set.
 require import Real.
 require import Distr.
 
+op map : ('a -> 'b) -> 'a set -> 'b set.
+axiom map_nil: forall (f:'a -> 'b),
+  map f Set.empty = Set.empty.
+axiom map_cons: forall (f:'a -> 'b) xs x,
+  mem x xs =>
+  map f xs = add (f x) (map f (rm x xs)).
+
 op fold_right : ('a -> 'b -> 'b) -> 'b -> 'a set -> 'b.
-axiom fold_nil: forall (e:'b) (f:'a -> 'b -> 'b),
+axiom fold_nil: forall (f:'a -> 'b -> 'b) (e:'b),
   fold_right f e Set.empty = e.
-axiom fold_cons: forall (e:'b) (f:'a -> 'b -> 'b) xs,
-  let x = Set.pick xs in
-  fold_right f e xs = f x (fold_right f e (Set.rm x xs)).
-axiom fold_cons2: forall (e:'b) (f:'a -> 'b -> 'b) xs x,
-  fold_right f e (add x xs) = f x (fold_right f e xs).
+axiom fold_rm: forall (f:'a -> 'b -> 'b) (e:'b) xs x,
+  mem x xs =>
+    fold_right f e xs = f x (fold_right f e (Set.rm x xs)).
+
+
+lemma mem_rm: forall (y:'a) (x:'a) (S:'a set),
+  x <> y =>
+  mem y (rm x S) = mem y S by [].
+
+lemma rm_add: forall (x:'a) (xs:'a set),
+  !(mem x xs) =>
+  rm x (add x xs) = xs by (intros _ _ _;apply Set.extensionality;trivial).
+
+lemma _map_add: forall (f:'a -> 'b) x xs,
+  !(mem x xs) =>
+  map f (add x xs) = add (f x) (map f xs).
+  intros f x xs h.
+  rewrite (map_cons<:'b, 'a> f (add x xs) x _);first trivial.
+  rewrite (_ : rm x (add x xs) = xs);first trivial.
+  split.
+save.
+
+lemma mem_map: forall (f:'a -> 'b) x xs,
+  mem x xs => mem (f x) (map f xs) by (intros _ _ S;elimT Set_ind S;trivial).
+
+lemma map_add: forall (f:'a -> 'b) x xs,
+  map f (add x xs) = add (f x) (map f xs).
+  intros f x xs.
+  case (mem x xs);last (apply _map_add;first assumption).
+  intros hh.
+  rewrite <- (mem_add<:'a> x xs _);first assumption.
+  rewrite <- (mem_add<:'b> (f x) (map f xs) _);trivial.
+save.
+
+lemma mem_map_bij: forall (f:'a -> 'b) x xs,
+  (forall x y, f x = f y => x = y) =>
+  mem x xs = mem (f x) (map f xs) by (intros _ _ S _;elimT Set.Set_ind S;trivial).
+
+lemma fold_add1: forall (f:'a -> 'b -> 'b) (e:'b) xs x,
+  !mem x xs =>
+    fold_right f e (add x xs) = f x (fold_right f e xs).
+  intros e f xs x.
+  rewrite (fold_rm<:'b, 'a> e f (add x xs) x _).
+  apply (add_mem x x xs).
+  intros h.
+  rewrite (rm_add<:'a> x xs _);[assumption|split].
+save.
+
+lemma fold_add2: forall (f:'a -> 'b -> 'b) (e:'b) xs x,
+  mem x xs =>
+    fold_right f e (add x xs) = fold_right f e xs by [].
+
+
 
 op sum(f:'a -> real, s:'a set) : real =
   fold_right (lambda (x:'a, sum:real), sum + f x) (0%r) s.
+
+lemma sum_nil:
+  forall (f:'a -> real), sum f Set.empty = 0%r by [].
+
+lemma sum_rm :
+  forall (f:'a -> real) (s:'a set) (x:'a),
+  mem x s =>
+  sum f s = (f x) + (sum f (rm x s)) by [].
+
+lemma sum_add :
+  forall (f:'a -> real) (s:'a set) (x:'a),
+  (!mem x s) =>
+  sum f (add x s) = (f x) + (sum f s) by [].
 
 lemma sum_in :
   forall (f:'a -> real) (s:'a set),
   sum f s = sum (lambda x, if mem x s then f x else 0%r) s.
 proof.
-admit.
+  delta sum.
+  simplify.
+  intros f s.
+  apply (Set.Set_ind
+(lambda S, S <= s => (
+fold_right (lambda (x : 'a) (sum : real), sum + f x) 0%r S =
+fold_right
+  (lambda (x : 'a) (sum : real), sum + if mem x s then f x else 0%r) 0%r
+  S)
+) _ _ s);first trivial.
+intros x S h hh hhh.
+simplify.
+rewrite (fold_add1<:real,'a> (lambda (x0 : 'a) (sum : real), sum + f x0) 0%r S x _);first assumption.
+rewrite (fold_add1<:real,'a> (lambda (x0 : 'a) (sum : real), sum + if mem x0 s then f x0 else 0%r) 0%r S x _);first assumption.
+simplify.
+rewrite (hh _);first trivial.
+cut lem : (mem x s = true);first trivial.
+rewrite lem.
+simplify.
+split.
 save.
 
-lemma sum_add :
+lemma sum_add2 :
   forall (f:'a -> real) (g:'a -> real) (s:'a set),
   (sum f s) + (sum g s) = sum (lambda x, f x + g x) s.
 proof.
-admit.
+intros f g s.
+delta sum.
+elimT Set_ind s;first trivial.
+intros x S h hh.
+simplify.
+rewrite (fold_add1<:real,'a> (lambda (x0 : 'a) (sum : real), sum + f x0) 0%r S x _);first assumption.
+rewrite (fold_add1<:real,'a> (lambda (x0 : 'a) (sum : real), sum + g x0) 0%r S x _);first assumption.
+rewrite (fold_add1<:real,'a> (lambda (x0 : 'a) (sum : real), sum + (f x0 + g x0)) 0%r S x _);first assumption.
+simplify.
+rewrite <- hh.
+generalize (fold_right (lambda (x0 : 'a) (sum : real), sum + f x0) 0%r S).
+generalize (fold_right (lambda (x0 : 'a) (sum : real), sum + g x0) 0%r S).
+intros a b.
+trivial.
+save.
+
+lemma sum_chind :
+  forall (f:'a -> real) (g:'a -> 'a) (gg:'a -> 'a) (s:'a set),
+    (forall x, g (gg x) = x /\ gg (g x) = x) => (*TROP FORT ?*)
+  (sum f s) = sum (lambda x, f (gg x)) (map g s).
+proof.
+intros f g gg s bij.
+delta sum.
+simplify.
+  apply (Set.Set_ind
+(lambda S, S <= s => (
+fold_right (lambda (x : 'a) (sum : real), sum + f x) 0%r S =
+fold_right (lambda (x : 'a) (sum : real), sum + f (gg x)) 0%r (map g S)
+)) _ _ s);first trivial.
+intros x S h hh.
+simplify.
+intros hhh.
+rewrite (_:map g (add x S) = add (g x) (map g S));first trivial.
+rewrite (fold_add1<:real,'a> (lambda (x0 : 'a) (sum : real), sum + f x0) 0%r S x _);first assumption.
+rewrite (fold_add1<:real,'a> (lambda (x0 : 'a) (sum : real), sum + f (gg x0)) 0%r (map g S) (g x) _);first (rewrite <- (mem_map_bij<:'a, 'a> g x S _);[trivial|assumption]).
+simplify.
+rewrite <- (hh _);first trivial.
+rewrite (_:gg (g x)=x);first trivial.
+split.
 save.
